Re-write heap lang semantics in an algebraic style
Similar to the Kleene-algebra transitions library, define a type of
transitions with some basic primitives and a general bind combinator,
then define everything as a function from an expression to this
transition denotation.

Transitions are expressed as an inductive to facilitate future exection
and extraction, but also have the obvious relational denotation. There's
currently a lot of duplication between the transitions (which are used
to write things down) and the relations (which are used in the proofs),
which we'll have to fix at some point. They might be unifiable with a
common typeclass.

While these are productive to write, we need to work out how to do
proofs with them. I'm hoping something like monadic/functor
simplification can cut through a lot of the helper definitions and
reduce things down to their essence (eg, you end up with fmaps and binds
of pure expressions all over the place, which can be reduced to a single
expression, or you have cases where there are multiple error checks in a
row that could be collapsed).

src/go_lang/lang.v
@@ -5,6 +5,7 @@ From stdpp Require Import gmap.
 From iris.algebra Require Export ofe.
 From iris.program_logic Require Export language ectx_language ectxi_language.
 From Perennial.Helpers Require Import CountableTactics.
+From Perennial.Helpers Require Import Transitions.
 From Perennial.program_logic Require Export crash_lang.
 From Perennial.go_lang Require Export locations.
 From Perennial Require Export Helpers.Integers.
@@ -910,14 +911,6 @@ Proof.
   rewrite right_id insert_union_singleton_l. done.
 Qed.
 
-Definition byte_vals : list byte -> list val :=
-   fmap (λ b, LitV (LitByte b)).
-
-Theorem byte_vals_length bs : length (byte_vals bs) = length bs.
-Proof.
-  rewrite /byte_vals fmap_length //.
-Qed.
-
 Definition is_Free {A} (mna: option (nonAtomic A)) := exists x, mna = Some (Free x).
 Global Instance is_Free_dec A (x: option (nonAtomic A)) : Decision (is_Free x).
 Proof.
@@ -935,117 +928,140 @@ Proof.
   destruct n; [ left; eauto | right; abstract (inversion 1) ].
 Defined.
 
-Inductive head_step : expr → state → list observation → expr → state → list expr → Prop :=
-  | RecS f x e σ :
-     head_step (Rec f x e) σ [] (Val $ RecV f x e) σ []
-  | PairS v1 v2 σ :
-     head_step (Pair (Val v1) (Val v2)) σ [] (Val $ PairV v1 v2) σ []
-  | InjLS v σ :
-     head_step (InjL $ Val v) σ [] (Val $ InjLV v) σ []
-  | InjRS v σ :
-     head_step (InjR $ Val v) σ [] (Val $ InjRV v) σ []
-  | BetaS f x e1 v2 e' σ :
-     e' = subst' x v2 (subst' f (RecV f x e1) e1) →
-     head_step (App (Val $ RecV f x e1) (Val v2)) σ [] e' σ []
-  | UnOpS op v v' σ :
-     un_op_eval op v = Some v' →
-     head_step (UnOp op (Val v)) σ [] (Val v') σ []
-  | BinOpS op v1 v2 v' σ :
-     bin_op_eval op v1 v2 = Some v' →
-     head_step (BinOp op (Val v1) (Val v2)) σ [] (Val v') σ []
-  | IfTrueS e1 e2 σ :
-     head_step (If (Val $ LitV $ LitBool true) e1 e2) σ [] e1 σ []
-  | IfFalseS e1 e2 σ :
-     head_step (If (Val $ LitV $ LitBool false) e1 e2) σ [] e2 σ []
-  | FstS v1 v2 σ :
-     head_step (Fst (Val $ PairV v1 v2)) σ [] (Val v1) σ []
-  | SndS v1 v2 σ :
-     head_step (Snd (Val $ PairV v1 v2)) σ [] (Val v2) σ []
-  | CaseLS v e1 e2 σ :
-     head_step (Case (Val $ InjLV v) e1 e2) σ [] (App e1 (Val v)) σ []
-  | CaseRS v e1 e2 σ :
-     head_step (Case (Val $ InjRV v) e1 e2) σ [] (App e2 (Val v)) σ []
-  | ForkS e σ:
-     head_step (Fork e) σ [] (Val $ LitV LitUnit) σ [e]
-  | AllocNS (n: u64) v σ l :
-     (0 < int.val n)%Z →
-     (∀ i, 0 ≤ i → i < int.val n → σ.(heap) !! (l +ₗ i) = None)%Z →
-     head_step (AllocN (Val $ LitV $ LitInt n) (Val v)) σ
-               []
-               (Val $ LitV $ LitLoc l) (state_init_heap l (int.val n) v σ)
-               []
-  | AllocStructS v σ l :
-     (∀ i, 0 ≤ i → i < length (flatten_struct v) → σ.(heap) !! (l +ₗ i) = None)%Z →
-     head_step (AllocStruct (Val v)) σ
-               []
-               (Val $ LitV $ LitLoc l) (state_insert_list l (flatten_struct v) σ)
-               []
-  | PrepareWriteS l v σ :
-     σ.(heap) !! l = Some $ Free v ->
-     head_step (PrepareWrite (Val $ LitV $ LitLoc l)) σ
-               []
-               (Val $ LitV $ LitUnit) (set heap <[l:=Writing]> σ)
-               []
-  | StartReadS l v n σ :
-     σ.(heap) !! l = Some $ Reading v n ->
-     head_step (StartRead (Val $ LitV $ LitLoc l)) σ
-               []
-               (of_val v) (set heap <[l:=Reading v (S n)]> σ)
-               []
-  | FinishReadS l v n σ :
-     σ.(heap) !! l = Some $ Reading v (S n) ->
-     head_step (StartRead (Val $ LitV $ LitLoc l)) σ
-               []
-               (Val $ LitV $ LitUnit) (set heap <[l:=Reading v n]> σ)
-               []
-  | LoadS l v σ :
-     σ.(heap) !! l = Some $ Free v →
-     head_step (Load (Val $ LitV $ LitLoc l)) σ [] (of_val v)
-               σ []
-  | FinishStoreS l v σ :
-     is_Writing (σ.(heap) !! l) ->
-     head_step (FinishStore (Val $ LitV $ LitLoc l) (Val v)) σ
-               []
-               (Val $ LitV LitUnit) (set heap <[l:=Free v]> σ)
-               []
-  | ExternalS op v σ v' σ' :
-     ext_step op v σ v' σ' ->
-     head_step (ExternalOp op (Val v)) σ
-               []
-               (Val v') σ'
-               []
-  | ObserveInputS selv σ :
-     let x := σ.(oracle) σ.(trace) selv in
-     let v := LitV $ LitInt $ x in
-     head_step (Input (Val selv)) σ
-               []
-               (Val v)
-               (set trace (add_event (In_ev selv v)) σ)
-               []
-  | ObserveOutputS v σ :
-     head_step (Output (Val v)) σ
-               []
-               (Val $ LitV LitUnit) (set trace (fun tr => add_event (Out_ev v) tr) σ)
-               []
-  | CmpXchgS l v1 v2 vl σ b :
-     σ.(heap) !! l = Some $ Free vl →
+Existing Instances r_mbind r_mret r_fmap.
+
+Definition ret_expr {state} (tr:transition state expr): transition state (list observation * expr * list expr) :=
+  (λ e, ([],e,[])) <$> tr.
+
+Definition ret_val {state} (v: val): transition state (list observation * expr * list expr) :=
+  ret ([], Val v, []).
+
+Definition ret_unit {state}: transition state (list observation * expr * list expr) :=
+  ret ([], Val (LitV LitUnit), []).
+
+Definition isFreshTo (bound:Z) (σ: state) (l: loc) :=
+  (forall i, 0 <= i -> i < bound -> σ.(heap) !! (l +ₗ i) = None)%Z.
+
+Instance alloc_gen bound : GenPred loc state (isFreshTo bound).
+Proof.
+  refine (fun _ σ => Some (exist _ (fresh_locs (dom (gset loc) σ.(heap))) _)).
+  hnf; intros.
+  apply (not_elem_of_dom (D := gset loc)).
+    by apply fresh_locs_fresh.
+Defined.
+
+Definition allocateN (bound:Z): transition state loc :=
+  suchThat (isFreshTo bound).
+
+Instance newProphId_gen: GenPred proph_id state (fun σ p => p ∉ σ.(used_proph_id)).
+Proof.
+  refine (fun _ σ => Some (exist _ (fresh σ.(used_proph_id)) _)).
+  apply is_fresh.
+Defined.
+
+Definition newProphId: transition state proph_id :=
+  suchThat (fun σ p => p ∉ σ.(used_proph_id)).
+
+Fixpoint head_trans (e: expr) :
+ transition state (list observation * expr * list expr) :=
+  match e with
+  | Rec f x e => ret_val $ RecV f x e
+  | Pair (Val v1) (Val v2) => ret_val $ PairV v1 v2
+  | InjL (Val v) => ret_val $ InjLV v
+  | InjR (Val v) => ret_val $ InjRV v
+  | App (Val (RecV f x e1)) (Val v2) =>
+    let e' := subst' x v2 (subst' f (RecV f x e1) e1) in
+    ret_expr $ ret e'
+  | UnOp op (Val v) => v' ← unwrap (un_op_eval op v); ret_val v'
+  | BinOp op (Val v1) (Val v2) => v' ← unwrap (bin_op_eval op v1 v2); ret_val v'
+  | If (Val (LitV (LitBool b))) e1 e2 => ret_expr (ret $ if b then e1 else e2)
+  | Fst (Val (PairV v1 v2)) => ret_val v1
+  | Snd (Val (PairV v1 v2)) => ret_val v2
+  | Case (Val (InjLV v)) e1 e2 => ret_expr (ret $ App e1 (Val v))
+  | Case (Val (InjRV v)) e1 e2 => ret_expr (ret $ App e2 (Val v))
+  | Fork e => ret ([], Val $ LitV LitUnit, [e])
+  | AllocN (Val (LitV (LitInt n))) (Val v) =>
+    check (0 < int.val n)%Z;;
+    l ← allocateN (int.val n);
+    modify (state_init_heap l (int.val n) v);;
+    ret_val (LitV $ LitLoc l)
+  | AllocStruct (Val v) =>
+    let vs := flatten_struct v in
+    l ← allocateN (Z.of_nat (length vs));
+    modify (state_insert_list l (flatten_struct v));;
+    ret_val (LitV $ LitLoc l)
+  | PrepareWrite (Val (LitV (LitLoc l))) =>
+    v ← reads (λ σ, σ.(heap) !! l) ≫= unwrap;
+      match v with
+      | Reading _ 0 =>
+        modify (set heap <[l:=Writing]>);;
+        ret_unit
+      | _ => undefined
+      end
+   | StartRead (Val (LitV (LitLoc l))) =>
+     nav ← reads (λ σ, σ.(heap) !! l) ≫= unwrap;
+     match nav with
+     | Reading v n =>
+       modify (set heap <[l:=Reading v (S n)]>);;
+       ret_val v
+     | _ => undefined
+     end
+   | FinishRead (Val (LitV (LitLoc l))) =>
+     nav ← reads (λ σ, σ.(heap) !! l) ≫= unwrap;
+     match nav with
+     | Reading v (S n) =>
+       modify (set heap <[l:=Reading v n]>);;
+       ret_unit
+     | _ => undefined
+     end
+   | Load (Val (LitV (LitLoc l))) =>
+     nav ← reads (λ σ, σ.(heap) !! l) ≫= unwrap;
+     match nav with
+     | Reading v 0 => ret_val v
+     | _ => undefined
+     end
+  | FinishStore (Val (LitV (LitLoc l))) (Val v) =>
+    nav ← reads (λ σ, σ.(heap) !! l);
+    check (is_Writing nav);;
+    modify (set heap <[l:=Free v]>);;
+    ret_unit
+  | ExternalOp op (Val v) => undefined (* TODO: need to change type of ext_step *)
+  | Input (Val selv) =>
+    x ← reads (λ σ, σ.(oracle) σ.(trace) selv);
+    let v := LitV $ LitInt $ x in
+    modify (set trace (add_event (In_ev selv v)));;
+    ret_val v
+  | Output (Val v) =>
+    modify (set trace (add_event (Out_ev v)));;
+    ret_unit
+  | CmpXchg (Val (LitV (LitLoc l))) (Val v1) (Val v2) =>
+    nav ← reads (λ σ, σ.(heap) !! l) ≫= unwrap;
+    match nav with
+    | Reading vl 0 =>
      (* Crucially, this compares the same way as [EqOp]! *)
-     vals_compare_safe vl v1 →
-     b = bool_decide (vl = v1) →
-     head_step (CmpXchg (Val $ LitV $ LitLoc l) (Val v1) (Val v2)) σ
-               []
-               (Val $ PairV vl (LitV $ LitBool b)) (if b then set heap <[l:=Free v2]> σ else σ)
-               []
-  | NewProphS σ p :
-     p ∉ σ.(used_proph_id) →
-     head_step NewProph σ
-               []
-               (Val $ LitV $ LitProphecy p) (set used_proph_id ({[ p ]} ∪.) σ)
-               []
-  | ResolveS p v e σ w σ' κs ts :
-     head_step e σ κs (Val v) σ' ts →
-     head_step (Resolve e (Val $ LitV $ LitProphecy p) (Val w)) σ
-               (κs ++ [(p, (v, w))]) (Val v) σ' ts.
+      check (vals_compare_safe vl v1);;
+      let b := bool_decide (vl = v1) in
+      ifThen b (modify (set heap <[l:=Free v2]>));;
+      ret_val (LitV $ LitBool b)
+    | _ => undefined
+    end
+  | NewProph =>
+    p ← newProphId;
+    modify (set used_proph_id ({[ p ]} ∪.));;
+    ret_val (LitV $ LitProphecy p)
+  | Resolve e (Val (LitV (LitProphecy p))) (Val w) =>
+    bind (head_trans e)
+         (fun '(κs,e',ts) =>
+            match e' with
+            | Val v => ret (κs ++ [(p, (v, w))], Val v, ts)
+            | _ => undefined
+            end)
+  | _ => undefined
+  end.
+
+Definition head_step: expr -> state -> list observation -> expr -> state -> list expr -> Prop :=
+  fun e s κs e' s' efs =>
+    relation.denote (head_trans e) s s' (κs, e', efs).
 
 (** Basic properties about the language *)
 Global Instance fill_item_inj Ki : Inj (=) (=) (fill_item Ki).
