src/Helpers/Transitions.v
@@ -1,0 +1,268 @@
+From Coq Require Import RelationClasses.
+From Coq Require Import Setoid.
+From Coq Require Import ZArith.
+
+From stdpp Require Import base.
+
+Set Implicit Arguments.
+Generalizable All Variables.
+
+Class GenPred T Σ (pred: Σ -> T -> Prop) := genNext : Z -> forall (s:Σ), option {x:T | pred s x}.
+Arguments GenPred : clear implicits.
+Notation GenType T Σ := (GenPred T Σ (fun _ _ => True)).
+
+Instance fallback_genPred T Σ p : GenPred T Σ p | 99 := fun _ _ => None.
+Instance bool_GenType Σ : GenType bool Σ := fun z _ => Some (exist _ (z mod 2 =? 0)%Z I).
+
+Section transition.
+  Context {Σ:Type}.
+
+  Inductive transition : Type -> Type :=
+  | runF {T} (f: Σ -> Σ * T) : transition T
+  | suchThat {T} (pred: Σ -> T -> Prop) {gen:GenPred T Σ pred} : transition T
+  | bind {T T'} (x: transition T') (rx: T' -> transition T) : transition T
+  .
+
+  Arguments suchThat {T} pred {gen}.
+
+  Definition ret {T} (v:T): transition T :=
+    runF (fun s => (s, v)).
+
+  Definition fmap {T1 T2} (f: T1 -> T2) (r: transition T1): transition T2 :=
+    bind r (fun x => ret (f x)).
+
+  Definition r_mbind : MBind transition :=
+    fun {A B} rx r => bind r rx.
+  Definition r_mret : MRet transition := @ret.
+  Definition r_fmap : FMap transition := @fmap.
+
+  Definition reads {T} (f: Σ -> T): transition T :=
+    runF (fun s => (s, f s)).
+
+  Definition modify (f: Σ -> Σ): transition unit :=
+    runF (fun s => (f s, tt)).
+
+  Definition any T {gen:GenType T Σ}: transition T :=
+    suchThat (fun _ _ => True).
+
+  Arguments any T {gen}.
+
+  Definition undefined {T}: transition T :=
+    suchThat (fun _ _ => False).
+
+  Definition plus {T} (r1 r2: transition T): transition T :=
+    bind (any bool) (fun b => if b then r1 else r2).
+
+  Definition check P `{!Decision P}: transition unit :=
+    if (decide P) then ret tt else undefined.
+
+  Definition checkNot P `{!Decision P}: transition unit :=
+    if (decide P) then undefined else ret tt.
+
+  Definition ifThen {T} P `{!Decision P} (r: transition T): transition T :=
+    if (decide P) then r else undefined.
+
+  Definition ifNot {T} P `{!Decision P} (r: transition T): transition T :=
+    if (decide P) then undefined else r.
+
+  Definition unwrap {T} (mx: option T): transition T :=
+    match mx with
+    | Some x => ret x
+    | None => undefined
+    end.
+
+  Definition next_hint (hints: list Z): Z * list Z :=
+    match hints with
+    | z::hints' => (z, hints')
+    | nil => (0%Z, nil)
+    end.
+
+  Fixpoint interpret (hints: list Z) {T} (tr: transition T): Σ -> option (list Z * Σ * T) :=
+    match tr with
+    | runF f => fun s => let (s', v) := f s in
+                     Some (hints, s', v)
+    | bind r1 rx => fun s => match interpret hints r1 s with
+                         | Some (hints', s', v) =>
+                           interpret hints' (rx v) s'
+                         | None => None
+                         end
+    | suchThat pred => let (hint, hints') := next_hint hints in
+                          fun s => match genNext hint s with
+                                | Some (exist _ x _) => Some (hints', s, x)
+                                | None => None
+                                end
+    end.
+
+End transition.
+
+Arguments transition Σ T : clear implicits.
+Arguments suchThat {Σ T} pred {gen}.
+Arguments any {Σ} T {gen}.
+Arguments check {Σ} P {_}.
+Arguments checkNot {Σ} P {_}.
+Arguments ifThen {Σ T} P {_}.
+Arguments ifNot {Σ T} P {_}.
+
+Module relation.
+  Section state.
+    Context (Σ:Type).
+    Definition t T := Σ -> Σ -> T -> Prop.
+
+    Inductive runF {T} (f:Σ -> Σ * T): t T :=
+    | runF_runs : forall s s' v,
+        f s = (s', v) ->
+        runF f s s' v.
+
+    Theorem runF_runs_to {T} (f: Σ -> Σ * T) s :
+      runF f s (fst (f s)) (snd (f s)).
+    Proof.
+      econstructor.
+      destruct (f s); auto.
+    Qed.
+
+    Inductive suchThat {T} (pred: Σ -> T -> Prop): t T :=
+    | suchThat_runs : forall s x,
+        pred s x ->
+        suchThat pred s s x
+    .
+
+    Inductive bind {T1 T2} (r: t T1) (rx: T1 -> t T2): t T2 :=
+    | bind_runs : forall s1 s2 x s3 x',
+        r s1 s2 x ->
+        (rx x) s2 s3 x' ->
+        bind r rx s1 s3 x'
+    .
+
+    Definition ret {T} (v:T): t T :=
+      runF (fun s => (s, v)).
+
+    Theorem inv_ret {T} (v:T) :
+      forall s1 s2 v', ret v s1 s2 v' ->
+                  s2 = s1 /\ v' = v.
+    Proof.
+      intros.
+      inversion H; subst.
+      inversion H0; subst.
+      auto.
+    Qed.
+
+    Definition fmap {T1 T2} (f: T1 -> T2) (r: t T1): t T2 :=
+      bind r (fun x => ret (f x)).
+
+    Fixpoint denote {T} (tr: transition Σ T): t T :=
+      match tr with
+      | Transitions.runF f => runF f
+      | Transitions.suchThat pred => suchThat pred
+      | Transitions.bind r rx => bind (denote r) (fun x => denote (rx x))
+      end.
+
+    Instance requiv {T}: Equiv (t T) :=
+      fun r1 r2 => forall s1 s2 v, r1 s1 s2 v <-> r2 s1 s2 v.
+
+    Ltac inv H :=
+      lazymatch type of H with
+      | ret _ _ _ _ => apply inv_ret in H; destruct H; subst
+      | _ => inversion H; subst; clear H
+      end.
+
+    Theorem interpret_sound {T} (tr: transition Σ T):
+      forall hints s s' hints' v,
+        interpret hints tr s = Some (hints', s', v) ->
+        denote tr s s' v.
+    Proof.
+      induction tr; simpl; intros.
+      - destruct_with_eqn (f s).
+        inv H.
+        eauto using runF_runs.
+      - destruct_with_eqn (next_hint hints).
+        destruct (genNext z s); [ | congruence ].
+        destruct s0.
+        inv H.
+        eauto using suchThat_runs.
+      - destruct_with_eqn (interpret hints tr s); [ | congruence ].
+        destruct p as [[hints'' s''] v'].
+        eapply IHtr in Heqo.
+        eapply H in H0.
+        econstructor; eauto.
+    Qed.
+
+    Global Instance equiv_Equiv T : Equivalence (@requiv T).
+    Proof.
+      constructor.
+      - firstorder.
+      - firstorder.
+      - intros r1 r2 r3.
+        unfold requiv; intros Heq1 Heq2 **.
+        rewrite Heq1.
+        apply Heq2.
+    Qed.
+
+    Theorem bind_id {T1 T2} (f: T1 -> t T2) x :
+      bind (ret x) f ≡ f x.
+    Proof.
+      intros s1 s2 v.
+      split; intros.
+      - inv H. inv H0.
+        auto.
+      - econstructor; eauto.
+        econstructor; eauto.
+    Qed.
+
+    Theorem bind_id' {T} (r: t T) :
+      bind r (fun x => ret x) ≡ r.
+    Proof.
+      intros s1 s2 v.
+      split; intros.
+      - inv H. inv H1.
+        auto.
+      - econstructor; eauto.
+        econstructor; eauto.
+    Qed.
+
+    Theorem bind_assoc {T1 T2 T3} (r1:  t T1) (r2: T1 -> t T2) (r3: T2 -> t T3) :
+      bind (bind r1 r2) r3 ≡ bind r1 (fun x => bind (r2 x) r3).
+    Proof.
+      intros s1 s2 v.
+      split; intros.
+      - inv H.
+        inv H0.
+        eauto using bind_runs.
+      - inv H.
+        inv H1.
+        eauto using bind_runs.
+    Qed.
+
+    Theorem fmap_ret T1 T2 (f: T1 -> T2) x :
+      fmap f (ret x) ≡ ret (f x).
+    Proof.
+      intros s1 s2 v.
+      split; intros.
+      - inv H.
+        inv H0.
+        inv H1.
+        econstructor; eauto.
+      - inv H.
+        econstructor; eauto.
+        { econstructor; eauto. }
+        { econstructor; eauto. }
+    Qed.
+
+    Global Instance bind_respects_equiv {T1 T2} :
+      Proper (requiv ==> pointwise_relation _ requiv ==> requiv) (@bind T1 T2).
+    Proof.
+      unfold Proper, respectful, pointwise_relation.
+      intros r1 r1' Heq1 r2 r2' Heq2.
+      intros s1 s2 v.
+      split; intros.
+      - inv H.
+        econstructor; eauto.
+        { eapply Heq1; eauto. }
+        { eapply Heq2; eauto. }
+      - inv H.
+        econstructor; eauto.
+        { eapply Heq1; eauto. }
+        { eapply Heq2; eauto. }
+    Qed.
+
+  End state.
+End relation.
